new approach: establish correctness while writing the code, using subset types

theories/dequeue_internal.v
@@ -1,9 +1,29 @@
-From Coq Require Import Program List ZArith.
+From Coq Require Import ssreflect.
+From Coq Require Import Program List ZArith Lia.
 Import ListNotations.
 From Equations Require Import Equations.
 Open Scope Z_scope.
+From Hammer Require Import Tactics.
 
-#[local] Obligation Tactic := try constructor.
+Fixpoint flattenp {A} (l: list (A * A)): list A :=
+  match l with
+  | [] => []
+  | (x, y) :: l' => x :: y :: flattenp l'
+  end.
+
+Lemma flattenp_app A (l1: list (A * A)) l2 : flattenp (l1 ++ l2) = flattenp l1 ++ flattenp l2.
+Proof. revert l2; induction l1; hauto. Qed.
+
+#[export] Hint Rewrite <-app_assoc : rlist.
+#[export] Hint Rewrite <-app_comm_cons : rlist.
+#[export] Hint Rewrite flattenp_app : rlist.
+#[export] Hint Rewrite app_nil_r : rlist.
+#[export] Hint Rewrite compose_id_right : rlist.
+
+#[local] Obligation Tactic :=
+  try first [ done | hauto db:rlist ].
+
+(* Types *)
 
 Inductive phantom : Type :=
   | PGreen
@@ -79,101 +99,6 @@ Inductive kont : Type -> phantom -> Type :=
   kont b is_green ->
   kont a is_red.
 
-Inductive s : Type -> Type :=
-| T : forall {a G Y},
-  kont a (PColor G Y PNotred) ->
-  s a.
-
-Equations green_prefix_cons {A : Type} : A -> buffer A is_green -> buffer A is_yellow :=
-green_prefix_cons x (B2 a b) := B3 x a b;
-green_prefix_cons x (B3 a b c) := B4 x a b c.
-
-Equations green_suffix_snoc {A : Type} : buffer A is_green -> A -> buffer A is_yellow :=
-green_suffix_snoc (B2 a b) x := B3 a b x;
-green_suffix_snoc (B3 a b c) x := B4 a b c x.
-
-Equations yellow_prefix_cons {A : Type} : A -> yellow_buffer A -> any_buffer A :=
-yellow_prefix_cons x (Yellowish buf) with buf => {
-  yellow_prefix_cons x _ (B1 a) := Any (B2 x a);
-  yellow_prefix_cons x _ (B2 a b) := Any (B3 x a b);
-  yellow_prefix_cons x _ (B3 a b c) := Any (B4 x a b c);
-  yellow_prefix_cons x _ (B4 a b c d) := Any (B5 x a b c d)
-}.
-
-Equations yellow_suffix_snoc {A : Type} : yellow_buffer A -> A -> any_buffer A :=
-yellow_suffix_snoc (Yellowish buf) x with buf := {
-  yellow_suffix_snoc _ x (B1 a) => Any (B2 a x);
-  yellow_suffix_snoc _ x (B2 a b) => Any (B3 a b x);
-  yellow_suffix_snoc _ x (B3 a b c) => Any (B4 a b c x);
-  yellow_suffix_snoc _ x (B4 a b c d) => Any (B5 a b c d x)
-}.
-
-Equations buffer_cons {A : Type} {C: phantom} : A -> buffer A C -> kont A is_green :=
-buffer_cons x B0 := Small (B1 x);
-buffer_cons x (B1 a) := Small (B2 x a);
-buffer_cons x (B2 a b) := Small (B3 x a b);
-buffer_cons x (B3 a b c) := Small (B4 x a b c);
-buffer_cons x (B4 a b c d) := Small (B5 x a b c d);
-buffer_cons x (B5 a b c d e) := G (Green (B3 x a b) HOLE (B3 c d e)) (Small B0).
-
-Equations buffer_snoc {A : Type} {C: phantom} : buffer A C -> A -> kont A is_green :=
-buffer_snoc B0 x := Small (B1 x);
-buffer_snoc (B1 a) x := Small (B2 a x);
-buffer_snoc (B2 a b) x := Small (B3 a b x);
-buffer_snoc (B3 a b c) x := Small (B4 a b c x);
-buffer_snoc (B4 a b c d) x := Small (B5 a b c d x);
-buffer_snoc (B5 a b c d e) x := G (Green (B3 a b c) HOLE (B3 d e x)) (Small B0).
-
-Equations green_uncons {A : Type} : buffer A is_green -> A * yellow_buffer A :=
-green_uncons (B2 a b) => (a, (Yellowish (B1 b)));
-green_uncons (B3 a b c) => (a, (Yellowish (B2 b c))).
-
-Equations green_unsnoc {A : Type} : buffer A is_green -> yellow_buffer A * A :=
-green_unsnoc (B2 a b) => ((Yellowish (B1 a)), b);
-green_unsnoc (B3 a b c) => ((Yellowish (B2 a b)), c).
-
-Equations yellow_uncons {A : Type} : yellow_buffer A -> A * any_buffer A :=
-yellow_uncons (Yellowish buf) with buf => {
-  yellow_uncons _ (B1 a) := (a, Any B0);
-  yellow_uncons _ (B2 a b) := (a, Any (B1 b));
-  yellow_uncons _ (B3 a b c) := (a, Any (B2 b c));
-  yellow_uncons _ (B4 a b c d) := (a, Any (B3 b c d))
-}.
-
-Equations yellow_unsnoc {A : Type} : yellow_buffer A -> any_buffer A * A :=
-yellow_unsnoc (Yellowish buf) with buf => {
-  yellow_unsnoc _ (B1 a) := (Any B0, a);
-  yellow_unsnoc _ (B2 a b) := (Any (B1 a), b);
-  yellow_unsnoc _ (B3 a b c) := (Any (B2 a b), c);
-  yellow_unsnoc _ (B4 a b c d) := (Any (B3 a b c), d)
-}.
-
-Equations buffer_uncons {A C} : buffer A C -> option (A * any_buffer A) :=
-buffer_uncons B0 := None;
-buffer_uncons (B5 a b c d e) := Some (a, Any (B4 b c d e));
-buffer_uncons buf := Some (yellow_uncons (Yellowish buf)).
-
-Equations buffer_unsnoc {A C} : buffer A C -> option (any_buffer A * A) :=
-buffer_unsnoc B0 := None;
-buffer_unsnoc (B5 a b c d e) := Some (Any (B4 a b c d), e);
-buffer_unsnoc buf := Some (yellow_unsnoc (Yellowish buf)).
-
-Equations prefix_rot {A C} : A -> buffer A C -> buffer A C * A :=
-prefix_rot x B0 := (B0, x);
-prefix_rot x (B1 a) := (B1 x, a);
-prefix_rot x (B2 a b) := (B2 x a, b);
-prefix_rot x (B3 a b c) := (B3 x a b, c);
-prefix_rot x (B4 a b c d) := (B4 x a b c, d);
-prefix_rot x (B5 a b c d e) := (B5 x a b c d, e).
-
-Equations suffix_rot {A C} : buffer A C -> A -> A * buffer A C :=
-suffix_rot B0 x := (x, B0);
-suffix_rot (B1 a) x := (a, B1 x);
-suffix_rot (B2 a b) x := (a, B2 b x);
-suffix_rot (B3 a b c) x := (a, B3 b c x);
-suffix_rot (B4 a b c d) x := (a, B4 b c d x);
-suffix_rot (B5 a b c d e) x := (a, B5 b c d e x).
-
 Inductive decompose (A : Type) : Type :=
 | Underflow : option A -> decompose A
 | Ok : buffer A is_green -> decompose A
@@ -183,290 +108,728 @@ Arguments Underflow {_}.
 Arguments Ok {_}.
 Arguments Overflow {_}.
 
-Equations prefix_decompose {A C} : buffer A C -> decompose A :=
-prefix_decompose B0 := Underflow None;
-prefix_decompose (B1 x) := Underflow (Some x);
-prefix_decompose (B2 a b) := Ok (B2 a b);
-prefix_decompose (B3 a b c) := Ok (B3 a b c);
-prefix_decompose (B4 a b c d) := Overflow (B2 a b) (c, d);
-prefix_decompose (B5 a b c d e) := Overflow (B3 a b c) (d, e).
-
-Equations suffix_decompose {A C} : buffer A C -> decompose A :=
-suffix_decompose B0 := Underflow None;
-suffix_decompose (B1 x) := Underflow (Some x);
-suffix_decompose (B2 a b) := Ok (B2 a b);
-suffix_decompose (B3 a b c) := Ok (B3 a b c);
-suffix_decompose (B4 a b c d) := Overflow (B2 c d) (a, b);
-suffix_decompose (B5 a b c d e) := Overflow (B3 c d e) (a, b).
-
-Equations prefix23 {A G Y} : option A -> A * A -> buffer A (PColor G Y PNotred) :=
-prefix23 None (b, c) := B2 b c;
-prefix23 (Some a) (b, c) := B3 a b c.
-
-Equations suffix23 {A G Y} : A * A -> option A -> buffer A (PColor G Y PNotred) :=
-suffix23 (a, b) None := B2 a b;
-suffix23 (a, b) (Some c) := B3 a b c.
-
-Equations prefix12 {A} : A -> option A -> buffer A is_yellow :=
-prefix12 x None := B1 x;
-prefix12 x (Some y) := B2 x y.
-
-Equations green_prefix_concat {A C} :
-  buffer A C -> buffer (A * A) is_green -> buffer A is_green * yellow_buffer (A * A) :=
-green_prefix_concat buf1 buf2 with (prefix_decompose buf1) => {
-  green_prefix_concat _ buf2 (Ok buf) => (buf, Yellowish buf2);
-  green_prefix_concat _ buf2 (Underflow opt) =>
-    let '(ab, buf) := green_uncons buf2 in
-    (prefix23 opt ab, buf);
-  green_prefix_concat _ buf2 (Overflow buf ab) =>
-    (buf, Yellowish (green_prefix_cons ab buf2))
-}.
-
-Equations green_suffix_concat {A C} :
-  buffer (A * A) is_green -> buffer A C -> yellow_buffer (A * A) * buffer A is_green :=
-green_suffix_concat buf1 buf2 with (suffix_decompose buf2) => {
-  green_suffix_concat buf1 _ (Ok buf) => (Yellowish buf1, buf);
-  green_suffix_concat buf1 _ (Underflow opt) =>
-    let '(buf, ab) := green_unsnoc buf1 in
-    (buf, (suffix23 ab opt));
-  green_suffix_concat buf1 _ (Overflow buf ab) =>
-    (Yellowish (green_suffix_snoc buf1 ab), buf)
-}.
-
-Equations prefix_concat {A B} :
-  buffer A B -> yellow_buffer (A * A) -> buffer A is_green * any_buffer (A * A) :=
-prefix_concat buf1 buf2 with prefix_decompose buf1 => {
-  prefix_concat _ (Yellowish buf2) (Ok buf) := (buf, Any buf2);
-  prefix_concat _ buf2 (Underflow opt) :=
-    let '(ab, buf) := yellow_uncons buf2 in
-    (prefix23 opt ab, buf);
-  prefix_concat _ buf2 (Overflow buf ab) :=
-    (buf, yellow_prefix_cons ab buf2)
-}.
-
-Equations suffix_concat {A B} :
-  yellow_buffer (A * A) -> buffer A B -> any_buffer (A * A) * buffer A is_green :=
-suffix_concat _ buf2 with suffix_decompose buf2 => {
-  suffix_concat (Yellowish buf1) _ (Ok buf) := (Any buf1, buf);
-  suffix_concat buf1 _ (Underflow opt) :=
-    let '(buf, ab) := yellow_unsnoc buf1 in
-    (buf, suffix23 ab opt);
-  suffix_concat buf1 _ (Overflow buf ab) :=
-    (yellow_suffix_snoc buf1 ab, buf)
-}.
-
-Inductive sandwich (A: Type) : Type :=
+Inductive sandwich (A : Type) : Type :=
 | Alone : option A -> sandwich A
 | Sandwich {C} : A -> buffer A C -> A -> sandwich A.
 Arguments Alone {A}.
 Arguments Sandwich {A C}.
 
-Equations buffer_unsandwich {A C} : buffer A C -> sandwich A :=
-buffer_unsandwich B0 := Alone None;
-buffer_unsandwich (B1 a) := Alone (Some a);
-buffer_unsandwich (B2 a b) := Sandwich a B0 b;
-buffer_unsandwich (B3 a b c) := Sandwich a (B1 b) c;
-buffer_unsandwich (B4 a b c d) := Sandwich a (B2 b c) d;
-buffer_unsandwich (B5 a b c d e) := Sandwich a (B3 b c d) e.
-
-Equations buffer_halve {A C} : buffer A C -> option A * any_buffer (A * A) :=
-buffer_halve B0 := (None, Any B0);
-buffer_halve (B1 a) := (Some a, Any B0);
-buffer_halve (B2 a b) := (None, Any (B1 (a, b)));
-buffer_halve (B3 a b c) := (Some a, Any (B1 (b, c)));
-buffer_halve (B4 a b c d) := (None, Any (B2 (a, b) (c, d)));
-buffer_halve (B5 a b c d e) := (Some a, Any (B2 (b, c) (d, e))).
-
-Equations kont_of_opt3 {A} : option A -> option (A * A) -> option A -> kont A is_green :=
-kont_of_opt3 None None None := Small B0;
-kont_of_opt3 (Some a) None None := Small (B1 a);
-kont_of_opt3 None None (Some a) := Small (B1 a);
-kont_of_opt3 (Some a) None (Some b) := Small (B2 a b);
-kont_of_opt3 None (Some (a, b)) None := Small (B2 a b);
-kont_of_opt3 (Some a) (Some (b, c)) None := Small (B3 a b c);
-kont_of_opt3 None (Some (a, b)) (Some c) := Small (B3 a b c);
-kont_of_opt3 (Some a) (Some (b, c)) (Some d) := Small (B4 a b c d).
-
-Equations make_small {A C1 C2 C3} :
-  buffer A C1 ->
-  buffer (A * A) C2 ->
-  buffer A C3 ->
-  kont A is_green :=
-make_small prefix1 buf suffix1 with (prefix_decompose prefix1), (suffix_decompose suffix1) => {
-make_small _ _ _ (Ok p1) (Ok s1) :=
-  G (Green p1 HOLE s1) (Small buf);
-make_small _ _ _ (Ok p1) (Underflow opt) with (buffer_unsnoc buf), opt => {
-  make_small _ _ _ _ _ None None := Small p1;
-  make_small _ _ _ _ _ None (Some x) := buffer_snoc p1 x;
-  make_small _ _ _ _ _ (Some (Any rest, cd)) _ :=
-    G (Green p1 HOLE (suffix23 cd opt)) (Small rest)
-  };
-make_small _ _ _ (Underflow opt) (Ok s1) with (buffer_uncons buf), opt => {
-  make_small _ _ _ _ _ None None := Small s1;
-  make_small _ _ _ _ _ None (Some x) := buffer_cons x s1;
-  make_small _ _ _ _ _ (Some (cd, Any rest)) _ :=
-    G (Green (prefix23 opt cd) HOLE s1) (Small rest)
-  };
-make_small _ _ _ (Underflow p1) (Underflow s1) with buffer_unsandwich buf => {
-  make_small _ _ _ _ _ (Sandwich ab rest cd) :=
-    G (Green (prefix23 p1 ab) HOLE (suffix23 cd s1)) (Small rest);
-  make_small _ _ _ _ _ (Alone opt) :=
-    kont_of_opt3 p1 opt s1;
- };
-make_small _ _ _ (Overflow p1 ab) (Ok s1) :=
-  G (Green p1 HOLE s1) (buffer_cons ab buf);
-make_small _ _ _ (Ok p1) (Overflow s1 ab) :=
-  G (Green p1 HOLE s1) (buffer_snoc buf ab);
-make_small _ _ _ (Underflow opt) (Overflow s1 ab) :=
-  let '(cd, center) := suffix_rot buf ab in
-  G (Green (prefix23 opt cd) HOLE s1) (Small center);
-make_small _ _ _ (Overflow p1 ab) (Underflow opt) :=
-  let '(center, cd) := prefix_rot ab buf in
-  G (Green p1 HOLE (suffix23 cd opt)) (Small center);
-make_small _ buf _ (Overflow p1 ab) (Overflow s1 cd) :=
-  let '(x, Any rest) := buffer_halve buf in
-  G (Green p1 (Yellow (prefix12 ab x) HOLE (B1 cd)) s1) (Small rest)
-}.
-
-Equations green_of_red {A : Type} : kont A is_red -> kont A is_green :=
-green_of_red (R (Red p1 HOLE s1) (Small buf)) :=
-  make_small p1 buf s1;
-green_of_red (R (Red p1 (Yellow p2 child s2) s1) k) :=
-  let '(p1, Any p2) := prefix_concat p1 (Yellowish p2) in
-  let '(Any s2, s1) := suffix_concat (Yellowish s2) s1 in
-  G (Green p1 HOLE s1) (R (Red p2 child s2) k);
-green_of_red (R (Red p1 HOLE s1) (G (Green p2 child s2) k)) :=
-  let '(p1, Yellowish p2) := green_prefix_concat p1 p2 in
-  let '(Yellowish s2, s1) := green_suffix_concat s2 s1 in
-    G (Green p1 (Yellow p2 child s2) s1) k.
-
 Inductive not_yellow : phantom -> Type :=
 | Not_yellow {G R} : not_yellow (PColor G PNotyellow R).
 
-Equations ensure_green {A C} : not_yellow C -> kont A C -> kont A is_green :=
-ensure_green Not_yellow (Small buf) := Small buf;
-ensure_green Not_yellow (G x k) := G x k;
+Inductive s : Type -> Type :=
+| T : forall {a G Y},
+  kont a (PColor G Y PNotred) ->
+  s a.
+
+(* Models *)
+
+Set Equations Transparent.
+
+Equations option_seq {A} : option A -> list A :=
+option_seq None := [];
+option_seq (Some x) := [x].
+
+Equations buffer_seq {A C} : buffer A C -> list A :=
+buffer_seq B0 := [];
+buffer_seq (B1 a) := [a];
+buffer_seq (B2 a b) := [a;b];
+buffer_seq (B3 a b c) := [a;b;c];
+buffer_seq (B4 a b c d) := [a;b;c;d];
+buffer_seq (B5 a b c d e) := [a;b;c;d;e].
+
+Equations yellow_buffer_seq {A} : yellow_buffer A -> list A :=
+yellow_buffer_seq (Yellowish buf) := buffer_seq buf.
+
+Equations any_buffer_seq {A} : any_buffer A -> list A :=
+any_buffer_seq (Any buf) := buffer_seq buf.
+
+Equations deque_front_seq {A B C K} : deque A B C K -> list A :=
+deque_front_seq HOLE := [];
+deque_front_seq (Yellow buf1 dq _) :=
+  buffer_seq buf1 ++ flattenp (deque_front_seq dq);
+deque_front_seq (Green buf1 dq _) :=
+  buffer_seq buf1 ++ flattenp (deque_front_seq dq);
+deque_front_seq (Red buf1 dq _) :=
+  buffer_seq buf1 ++ flattenp (deque_front_seq dq).
+
+Equations deque_rear_seq {A B C K} : deque A B C K -> list A :=
+deque_rear_seq HOLE := [];
+deque_rear_seq (Yellow _ dq buf2) :=
+  flattenp (deque_rear_seq dq) ++ buffer_seq buf2;
+deque_rear_seq (Green _ dq buf2) :=
+  flattenp (deque_rear_seq dq) ++ buffer_seq buf2;
+deque_rear_seq (Red _ dq buf2) :=
+  flattenp (deque_rear_seq dq) ++ buffer_seq buf2.
+
+Equations deque_hole_flatten {A B C K} : deque A B C K -> list B -> list A :=
+deque_hole_flatten HOLE := id;
+deque_hole_flatten (Yellow _ dq _) :=
+  flattenp ∘ deque_hole_flatten dq;
+deque_hole_flatten (Green _ dq _) :=
+  flattenp ∘ deque_hole_flatten dq;
+deque_hole_flatten (Red _ dq _) :=
+  flattenp ∘ deque_hole_flatten dq.
+
+Equations kont_seq {A C} : kont A C -> list A :=
+kont_seq (Small buf) := buffer_seq buf;
+kont_seq (G dq kont) :=
+  deque_front_seq dq ++
+  deque_hole_flatten dq (kont_seq kont) ++
+  deque_rear_seq dq;
+kont_seq (Y dq kont) :=
+  deque_front_seq dq ++
+  deque_hole_flatten dq (kont_seq kont) ++
+  deque_rear_seq dq;
+kont_seq (R dq kont) :=
+  deque_front_seq dq ++
+  deque_hole_flatten dq (kont_seq kont) ++
+  deque_rear_seq dq.
+
+Equations decompose_main_seq {A : Type} (dec : decompose A) : list A :=
+decompose_main_seq (Underflow None) := [];
+decompose_main_seq (Underflow (Some x)) := [x];
+decompose_main_seq (Ok b) := buffer_seq b;
+decompose_main_seq (Overflow b _) := buffer_seq b.
+
+Equations decompose_rest_seq {A : Type} (dec : decompose A) : list A :=
+decompose_rest_seq (Underflow _) := [];
+decompose_rest_seq (Ok _) := [];
+decompose_rest_seq (Overflow b (x, y)) := [x; y].
+
+Equations sandwich_seq {A : Type} (sw : sandwich A) : list A :=
+sandwich_seq (Alone None) := [];
+sandwich_seq (Alone (Some x)) := [x];
+sandwich_seq (Sandwich x b y) := x :: buffer_seq b ++ [y].
+
+Equations s_seq {A} : s A -> list A :=
+s_seq (T kont) := kont_seq kont.
+
+Unset Equations Transparent.
+
+(* Functions *)
+
+Notation "? x" := (@exist _ _ x _) (at level 100).
+
+Equations green_prefix_cons {A : Type} (x : A) (b : buffer A is_green) :
+  { b' : buffer A is_yellow | buffer_seq b' = x :: buffer_seq b } :=
+green_prefix_cons x (B2 a b) := ? B3 x a b;
+green_prefix_cons x (B3 a b c) := ? B4 x a b c.
+
+Equations green_suffix_snoc {A : Type} (b : buffer A is_green) (x : A) :
+  { b' : buffer A is_yellow | buffer_seq b' = buffer_seq b ++ [x] } :=
+green_suffix_snoc (B2 a b) x := ? B3 a b x;
+green_suffix_snoc (B3 a b c) x := ? B4 a b c x.
+
+Equations yellow_prefix_cons {A : Type} (x : A) (b : yellow_buffer A) :
+  { b' : any_buffer A | any_buffer_seq b' = x :: yellow_buffer_seq b } :=
+yellow_prefix_cons x (Yellowish buf) with buf => {
+  yellow_prefix_cons x _ (B1 a) := ? Any (B2 x a);
+  yellow_prefix_cons x _ (B2 a b) := ? Any (B3 x a b);
+  yellow_prefix_cons x _ (B3 a b c) := ? Any (B4 x a b c);
+  yellow_prefix_cons x _ (B4 a b c d) := ? Any (B5 x a b c d)
+}.
+
+Equations yellow_suffix_snoc {A : Type} (b : yellow_buffer A) (x : A) :
+  { b' : any_buffer A | any_buffer_seq b' = yellow_buffer_seq b ++ [x] } :=
+yellow_suffix_snoc (Yellowish buf) x with buf := {
+  yellow_suffix_snoc _ x (B1 a) => ? Any (B2 a x);
+  yellow_suffix_snoc _ x (B2 a b) => ? Any (B3 a b x);
+  yellow_suffix_snoc _ x (B3 a b c) => ? Any (B4 a b c x);
+  yellow_suffix_snoc _ x (B4 a b c d) => ? Any (B5 a b c d x)
+}.
+
+Equations buffer_cons {A : Type} {C : phantom} (x : A) (b : buffer A C) :
+  { k : kont A is_green | kont_seq k = x :: buffer_seq b } :=
+buffer_cons x B0 := ? Small (B1 x);
+buffer_cons x (B1 a) := ? Small (B2 x a);
+buffer_cons x (B2 a b) := ? Small (B3 x a b);
+buffer_cons x (B3 a b c) := ? Small (B4 x a b c);
+buffer_cons x (B4 a b c d) := ? Small (B5 x a b c d);
+buffer_cons x (B5 a b c d e) := ? G (Green (B3 x a b) HOLE (B3 c d e)) (Small B0).
+
+Equations buffer_snoc {A : Type} {C : phantom} (b : buffer A C) (x : A) :
+  { k : kont A is_green | kont_seq k = buffer_seq b ++ [x] } :=
+buffer_snoc B0 x := ? Small (B1 x);
+buffer_snoc (B1 a) x := ? Small (B2 a x);
+buffer_snoc (B2 a b) x := ? Small (B3 a b x);
+buffer_snoc (B3 a b c) x := ? Small (B4 a b c x);
+buffer_snoc (B4 a b c d) x := ? Small (B5 a b c d x);
+buffer_snoc (B5 a b c d e) x := ? G (Green (B3 a b c) HOLE (B3 d e x)) (Small B0).
+
+Equations green_uncons {A : Type} (b : buffer A is_green) :
+  { '(x, b') : A * yellow_buffer A | buffer_seq b = x :: yellow_buffer_seq b' } :=
+green_uncons (B2 a b) => ? (a, (Yellowish (B1 b)));
+green_uncons (B3 a b c) => ? (a, (Yellowish (B2 b c))).
+
+Equations green_unsnoc {A : Type} (b : buffer A is_green) :
+  { '(b', x) : yellow_buffer A * A | buffer_seq b = yellow_buffer_seq b' ++ [x] } :=
+green_unsnoc (B2 a b) => ? ((Yellowish (B1 a)), b);
+green_unsnoc (B3 a b c) => ? ((Yellowish (B2 a b)), c).
+
+Equations yellow_uncons {A : Type} (b : yellow_buffer A) :
+  { '(x, b') : A * any_buffer A | yellow_buffer_seq b = x :: any_buffer_seq b' } :=
+yellow_uncons (Yellowish buf) with buf => {
+  yellow_uncons _ (B1 a) := ? (a, Any B0);
+  yellow_uncons _ (B2 a b) := ? (a, Any (B1 b));
+  yellow_uncons _ (B3 a b c) := ? (a, Any (B2 b c));
+  yellow_uncons _ (B4 a b c d) := ? (a, Any (B3 b c d))
+}.
+
+Equations yellow_unsnoc {A : Type} (b : yellow_buffer A) :
+  { '(b', x) : any_buffer A * A | yellow_buffer_seq b = any_buffer_seq b' ++ [x] } :=
+yellow_unsnoc (Yellowish buf) with buf => {
+  yellow_unsnoc _ (B1 a) := ? (Any B0, a);
+  yellow_unsnoc _ (B2 a b) := ? (Any (B1 a), b);
+  yellow_unsnoc _ (B3 a b c) := ? (Any (B2 a b), c);
+  yellow_unsnoc _ (B4 a b c d) := ? (Any (B3 a b c), d)
+}.
+
+Equations buffer_uncons {A C} (b : buffer A C) :
+  { o : option (A * any_buffer A) |
+    buffer_seq b =
+    match o with
+    | None => []
+    | Some (x, b') => x :: any_buffer_seq b'
+    end } :=
+buffer_uncons B0 := ? None;
+buffer_uncons (B5 a b c d e) := ? Some (a, Any (B4 b c d e));
+buffer_uncons buf with yellow_uncons (Yellowish buf) => { | ? o := ? Some o }.
+
+Equations buffer_unsnoc {A C} (b : buffer A C) :
+  { o : option (any_buffer A * A) |
+    buffer_seq b =
+    match o with
+    | None => []
+    | Some (b', x) => any_buffer_seq b' ++ [x]
+    end } :=
+buffer_unsnoc B0 := ? None;
+buffer_unsnoc (B5 a b c d e) := ? Some (Any (B4 a b c d), e);
+buffer_unsnoc buf with yellow_unsnoc (Yellowish buf) => { | ? o := ? Some o }.
+
+Equations prefix_rot {A C} (x : A) (b : buffer A C) :
+  { '(b', y) : buffer A C * A | x :: buffer_seq b = buffer_seq b' ++ [y] } :=
+prefix_rot x B0 := ? (B0, x);
+prefix_rot x (B1 a) := ? (B1 x, a);
+prefix_rot x (B2 a b) := ? (B2 x a, b);
+prefix_rot x (B3 a b c) := ? (B3 x a b, c);
+prefix_rot x (B4 a b c d) := ? (B4 x a b c, d);
+prefix_rot x (B5 a b c d e) := ? (B5 x a b c d, e).
+
+Equations suffix_rot {A C} (b : buffer A C) (y : A) :
+  { '(x, b') : A * buffer A C | buffer_seq b ++ [y] = x :: buffer_seq b' } :=
+suffix_rot B0 x := ? (x, B0);
+suffix_rot (B1 a) x := ? (a, B1 x);
+suffix_rot (B2 a b) x := ? (a, B2 b x);
+suffix_rot (B3 a b c) x := ? (a, B3 b c x);
+suffix_rot (B4 a b c d) x := ? (a, B4 b c d x);
+suffix_rot (B5 a b c d e) x := ? (a, B5 b c d e x).
+
+Equations prefix_decompose {A C} (b : buffer A C) :
+  { dec : decompose A | buffer_seq b = decompose_main_seq dec ++ decompose_rest_seq dec } :=
+prefix_decompose B0 := ? Underflow None;
+prefix_decompose (B1 x) := ? Underflow (Some x);
+prefix_decompose (B2 a b) := ? Ok (B2 a b);
+prefix_decompose (B3 a b c) := ? Ok (B3 a b c);
+prefix_decompose (B4 a b c d) := ? Overflow (B2 a b) (c, d);
+prefix_decompose (B5 a b c d e) := ? Overflow (B3 a b c) (d, e).
+
+Equations suffix_decompose {A C} (b : buffer A C) :
+  { dec : decompose A | buffer_seq b = decompose_rest_seq dec ++ decompose_main_seq dec } :=
+suffix_decompose B0 := ? Underflow None;
+suffix_decompose (B1 x) := ? Underflow (Some x);
+suffix_decompose (B2 a b) := ? Ok (B2 a b);
+suffix_decompose (B3 a b c) := ? Ok (B3 a b c);
+suffix_decompose (B4 a b c d) := ? Overflow (B2 c d) (a, b);
+suffix_decompose (B5 a b c d e) := ? Overflow (B3 c d e) (a, b).
+
+Equations prefix23 {A G Y} (o : option A) (p: A * A) :
+  { b : buffer A (PColor G Y PNotred) |
+    let '(y, z) := p in
+    buffer_seq b = option_seq o ++ [y; z] } :=
+prefix23 None (b, c) := ? B2 b c;
+prefix23 (Some a) (b, c) := ? B3 a b c.
+
+Equations suffix23 {A G Y} (p : A * A) (o : option A) :
+  { b : buffer A (PColor G Y PNotred) |
+    let '(x, y) := p in
+    buffer_seq b = [x; y] ++ option_seq o } :=
+suffix23 (a, b) None := ? B2 a b;
+suffix23 (a, b) (Some c) := ? B3 a b c.
+
+Equations prefix12 {A} (x : A) (o : option A) :
+  { b : buffer A is_yellow | buffer_seq b = x :: option_seq o } :=
+prefix12 x None := ? B1 x;
+prefix12 x (Some y) := ? B2 x y.
+
+Equations green_prefix_concat {A C}
+  (buf1 : buffer A C)
+  (buf2 : buffer (A * A) is_green) :
+  { '(buf1', buf2') : buffer A is_green * yellow_buffer (A * A) |
+    buffer_seq buf1 ++ flattenp (buffer_seq buf2) =
+    buffer_seq buf1' ++ flattenp (yellow_buffer_seq buf2') } :=
+green_prefix_concat buf1 buf2 with prefix_decompose buf1 => {
+  | (? Ok buf) => ? (buf, Yellowish buf2);
+  | (? Underflow opt) with green_uncons buf2 => {
+    | (? (ab, buf)) =>
+        let '(? prefix) := prefix23 opt ab in
+        ? (prefix, buf) };
+  | (? Overflow buf ab) =>
+    let '(? suffix) := green_prefix_cons ab buf2 in
+    ? (buf, Yellowish suffix)
+}.
+
+Equations green_suffix_concat {A C}
+  (buf1 : buffer (A * A) is_green)
+  (buf2 : buffer A C) :
+  { '(buf1', buf2') : yellow_buffer (A * A) * buffer A is_green |
+    flattenp (buffer_seq buf1) ++ buffer_seq buf2 =
+    flattenp (yellow_buffer_seq buf1') ++ buffer_seq buf2' } :=
+green_suffix_concat buf1 buf2 with suffix_decompose buf2 => {
+  | ? Ok buf => ? (Yellowish buf1, buf);
+  | ? Underflow opt with green_unsnoc buf1 => {
+    | ? (buf, ab) =>
+        let '(? suffix) := suffix23 ab opt in
+        ? (buf, suffix) };
+  | ? Overflow buf ab =>
+    let '(? prefix) := green_suffix_snoc buf1 ab in
+    ? (Yellowish prefix, buf)
+}.
+
+Equations prefix_concat {A B}
+  (buf1 : buffer A B)
+  (buf2 : yellow_buffer (A * A)) :
+  { '(buf1', buf2') : buffer A is_green * any_buffer (A * A) |
+    buffer_seq buf1 ++ flattenp (yellow_buffer_seq buf2) =
+    buffer_seq buf1' ++ flattenp (any_buffer_seq buf2') } :=
+prefix_concat buf1 buf2 with prefix_decompose buf1 => {
+  | ? (Ok buf) =>
+    let '(Yellowish buf2) := buf2 in
+    ? (buf, Any buf2);
+  | ? (Underflow opt) with yellow_uncons buf2 => {
+    | ? (ab, buf) =>
+      let '(? prefix) := prefix23 opt ab in
+      ? (prefix, buf) };
+  | ? (Overflow buf ab) =>
+    let '(? suffix) := yellow_prefix_cons ab buf2 in
+    ? (buf, suffix)
+}.
+
+Equations suffix_concat {A B}
+  (buf1 : yellow_buffer (A * A))
+  (buf2 : buffer A B) :
+  { '(buf1', buf2') : any_buffer (A * A) * buffer A is_green |
+    flattenp (yellow_buffer_seq buf1) ++ buffer_seq buf2 =
+    flattenp (any_buffer_seq buf1') ++ buffer_seq buf2' } :=
+suffix_concat buf1 buf2 with suffix_decompose buf2 => {
+  | ? (Ok buf) =>
+    let '(Yellowish buf1) := buf1 in
+    ? (Any buf1, buf);
+  | ? (Underflow opt) with yellow_unsnoc buf1 => {
+    | ? (buf, ab) =>
+      let '(? suffix) := suffix23 ab opt in
+      ? (buf, suffix) };
+  | ? (Overflow buf ab) =>
+    let '(? prefix) := yellow_suffix_snoc buf1 ab in
+    ? (prefix, buf)
+}.
+
+Equations buffer_unsandwich {A C} (b : buffer A C) :
+  { sw : sandwich A | buffer_seq b = sandwich_seq sw } :=
+buffer_unsandwich B0 := ? Alone None;
+buffer_unsandwich (B1 a) := ? Alone (Some a);
+buffer_unsandwich (B2 a b) := ? Sandwich a B0 b;
+buffer_unsandwich (B3 a b c) := ? Sandwich a (B1 b) c;
+buffer_unsandwich (B4 a b c d) := ? Sandwich a (B2 b c) d;
+buffer_unsandwich (B5 a b c d e) := ? Sandwich a (B3 b c d) e.
+
+Equations buffer_halve {A C} (b : buffer A C) :
+  { '(o, b') : option A * any_buffer (A * A) |
+    buffer_seq b = option_seq o ++ flattenp (any_buffer_seq b') } :=
+buffer_halve B0 := ? (None, Any B0);
+buffer_halve (B1 a) := ? (Some a, Any B0);
+buffer_halve (B2 a b) := ? (None, Any (B1 (a, b)));
+buffer_halve (B3 a b c) := ? (Some a, Any (B1 (b, c)));
+buffer_halve (B4 a b c d) := ? (None, Any (B2 (a, b) (c, d)));
+buffer_halve (B5 a b c d e) := ? (Some a, Any (B2 (b, c) (d, e))).
+
+Equations kont_of_opt3 {A} (o1 : option A) (o2 : option (A * A)) (o3 : option A) :
+  { k : kont A is_green |
+    kont_seq k = option_seq o1 ++ flattenp (option_seq o2) ++ option_seq o3 } :=
+kont_of_opt3 None None None := ? Small B0;
+kont_of_opt3 (Some a) None None := ? Small (B1 a);
+kont_of_opt3 None None (Some a) := ? Small (B1 a);
+kont_of_opt3 (Some a) None (Some b) := ? Small (B2 a b);
+kont_of_opt3 None (Some (a, b)) None := ? Small (B2 a b);
+kont_of_opt3 (Some a) (Some (b, c)) None := ? Small (B3 a b c);
+kont_of_opt3 None (Some (a, b)) (Some c) := ? Small (B3 a b c);
+kont_of_opt3 (Some a) (Some (b, c)) (Some d) := ? Small (B4 a b c d).
+
+Equations make_small {A C1 C2 C3}
+  (b1 : buffer A C1)
+  (b2 : buffer (A * A) C2)
+  (b3 : buffer A C3) :
+  { k : kont A is_green |
+    kont_seq k = buffer_seq b1 ++ flattenp (buffer_seq b2) ++ buffer_seq b3 } :=
+make_small prefix1 buf suffix1 with (prefix_decompose prefix1), (suffix_decompose suffix1) => {
+  | (? Ok p1), (? Ok s1) :=
+    ? G (Green p1 HOLE s1) (Small buf);
+  | (? Ok p1), (? Underflow opt) with buffer_unsnoc buf => {
+    | ? None with opt => {
+      | None := ? Small p1;
+      | Some x with buffer_snoc p1 x => { | ? k := ? k } };
+    | ? Some (Any rest, cd) with suffix23 cd opt => {
+      | ? suffix := ? G (Green p1 HOLE suffix) (Small rest) }
+  };
+  | (? Underflow opt), (? Ok s1) with buffer_uncons buf => {
+    | ? None with opt => {
+      | None := ? Small s1;
+      | Some x with buffer_cons x s1 => { | ? k := ? k } };
+    | ? Some (cd, Any rest) with prefix23 opt cd => {
+      | ? prefix := ? G (Green prefix HOLE s1) (Small rest) }
+  };
+  | (? Underflow p1), (? Underflow s1) with buffer_unsandwich buf => {
+    | ? Sandwich ab rest cd with prefix23 p1 ab, suffix23 cd s1 => {
+      | ? prefix, ? suffix := ? G (Green prefix HOLE suffix) (Small rest) };
+    | ? Alone opt with kont_of_opt3 p1 opt s1 => { | ? k := ? k } }
+  | (? Overflow p1 ab), (? Ok s1) with buffer_cons ab buf => {
+    | ? rest => ? G (Green p1 HOLE s1) rest };
+  | (? Ok p1), (? Overflow s1 ab) with buffer_snoc buf ab => {
+    | ? rest => ? G (Green p1 HOLE s1) rest };
+  | (? Underflow opt), (? Overflow s1 ab) with suffix_rot buf ab => {
+    | ? (cd, center) with prefix23 opt cd => {
+      | ? prefix => ? G (Green prefix HOLE s1) (Small center) } };
+  | (? Overflow p1 ab), (? Underflow opt) with prefix_rot ab buf => {
+    | ? (center, cd) with suffix23 cd opt => {
+      | ? suffix => ? G (Green p1 HOLE suffix) (Small center) } };
+  | (? Overflow p1 ab), (? Overflow s1 cd) with buffer_halve buf => {
+    | ? (x, Any rest) with prefix12 ab x => {
+      | ? prefix => ? G (Green p1 (Yellow prefix HOLE (B1 cd)) s1) (Small rest) } }
+}.
+Next Obligation.
+  cbn. intros * Hpre1 * Hcenter%(f_equal flattenp) Hsuff * Hpre.
+  destruct ab; destruct cd; autorewrite with rlist in *; cbn in *.
+  rewrite Hpre. autorewrite with rlist; cbn.
+  rewrite (_ : forall l1 x y l2, x :: y :: l1 ++ l2 = (x :: y :: l1) ++ l2) //.
+  rewrite -Hcenter. hauto db:rlist.
+Qed.
+Next Obligation.
+  cbn. intros * Hpre1 * Hcenter%(f_equal flattenp) * Hsuff1 * Hsuff.
+  destruct ab; destruct cd; autorewrite with rlist in *; cbn in *.
+  rewrite Hpre1. autorewrite with rlist; cbn.
+  rewrite (_ : forall l1 x y l2, x :: y :: l1 ++ l2 = (x :: y :: l1) ++ l2) //.
+  rewrite Hcenter. hauto db:rlist.
+Qed.
+
+Equations green_of_red {A : Type} (k : kont A is_red) :
+  { k' : kont A is_green | kont_seq k' = kont_seq k } :=
+green_of_red (R (Red p1 HOLE s1) (Small buf)) with make_small p1 buf s1 => {
+  | ? k' := ? k' };
+green_of_red (R (Red p1 (Yellow p2 child s2) s1) k)
+  with prefix_concat p1 (Yellowish p2), suffix_concat (Yellowish s2) s1 => {
+  | ? (p1', Any p2'), ? (Any s2', s1') :=
+    ? G (Green p1' HOLE s1') (R (Red p2' child s2') k) };
+green_of_red (R (Red p1 HOLE s1) (G (Green p2 child s2) k))
+  with green_prefix_concat p1 p2, green_suffix_concat s2 s1 => {
+  | ? (p1', Yellowish p2'), ? (Yellowish s2', s1') :=
+    ? G (Green p1' (Yellow p2' child s2') s1') k }.
+Next Obligation.
+  cbn. intros * H1 * H2 *. autorewrite with rlist.
+  rewrite !app_assoc H1. hauto db:rlist.
+Qed.
+Next Obligation.
+  cbn. intros * H1 * H2 *. autorewrite with rlist.
+  rewrite !app_assoc H1. hauto db:rlist.
+Qed.
+
+Equations ensure_green {A C} (ny: not_yellow C) (k : kont A C) :
+  { k' : kont A is_green | kont_seq k' = kont_seq k } :=
+ensure_green Not_yellow (Small buf) := ? Small buf;
+ensure_green Not_yellow (G x k) := ? G x k;
 ensure_green Not_yellow (R x k) := green_of_red (R x k).
 
-Equations yellow {A B: Type} {G1 Y1 Y2 K2 G3 Y3 G4 R4 : phantom} :
-  buffer A (PColor G1 Y1 PNotred) ->
-  deque (A * A) B (PColor PNotgreen Y2 PNotred) K2 ->
-  buffer A (PColor G3 Y3 PNotred) ->
-  kont B (PColor G4 PNotyellow R4) ->
-  s A
+Equations yellow {A B: Type} {G1 Y1 Y2 K2 G3 Y3 G4 R4 : phantom}
+  (buf1 : buffer A (PColor G1 Y1 PNotred))
+  (dq : deque (A * A) B (PColor PNotgreen Y2 PNotred) K2)
+  (buf2 : buffer A (PColor G3 Y3 PNotred))
+  (k : kont B (PColor G4 PNotyellow R4)) :
+  { sq : s A |
+    s_seq sq = buffer_seq buf1 ++
+               flattenp (deque_front_seq dq) ++
+               flattenp (deque_hole_flatten dq (kont_seq k)) ++
+               flattenp (deque_rear_seq dq) ++
+               buffer_seq buf2 }
 :=
-yellow p1 child s1 k := T (Y (Yellow p1 child s1) (ensure_green Not_yellow k)).
+yellow p1 child s1 k with ensure_green Not_yellow k => {
+  | ? k' => ? T (Y (Yellow p1 child s1) k') }.
 
-Equations red {A B: Type} {C1 Y2 K2 C3 : phantom} :
-  buffer A C1 ->
-  deque (A * A) B (PColor PNotgreen Y2 PNotred) K2 ->
-  buffer A C3 ->
-  kont B is_green ->
-  s A
+Equations red {A B: Type} {C1 Y2 K2 C3 : phantom}
+  (buf1 : buffer A C1)
+  (dq : deque (A * A) B (PColor PNotgreen Y2 PNotred) K2)
+  (buf2 : buffer A C3)
+  (k : kont B is_green) :
+  { sq : s A |
+    s_seq sq = buffer_seq buf1 ++
+               flattenp (deque_front_seq dq) ++
+               flattenp (deque_hole_flatten dq (kont_seq k)) ++
+               flattenp (deque_rear_seq dq) ++
+               buffer_seq buf2 }
 :=
-red p1 child s1 k := T (green_of_red (R (Red p1 child s1) k)).
+red p1 child s1 k with green_of_red (R (Red p1 child s1) k) => {
+  | ? k' => ? T k' }.
 
 Module S.
 
-Equations cons {A: Type} : A -> s A -> s A :=
-cons x (T (Small buf)) :=
-  T (buffer_cons x buf);
-cons x (T (G (Green p1 child s1) kont)) :=
-  yellow (green_prefix_cons x p1) child s1 kont;
-cons x (T (Y (Yellow p1 child s1) kont)) :=
-  let 'Any p1 := yellow_prefix_cons x (Yellowish p1) in
-  red p1 child s1 kont.
+Equations cons {A: Type} (x : A) (sq : s A) :
+  { sq' : s A | s_seq sq' = x :: s_seq sq }
+:=
+cons x (T (Small buf)) with buffer_cons x buf => {
+  | ? buf' => ? T buf' };
+cons x (T (G (Green p1 child s1) kont)) with green_prefix_cons x p1 => {
+  | ? buf' with yellow buf' child s1 kont => {
+    | ? sq' => ? sq' } };
+cons x (T (Y (Yellow p1 child s1) kont))
+  with yellow_prefix_cons x (Yellowish p1) => {
+  | ? (Any p1') with red p1' child s1 kont => {
+    | ? sq' => ? sq' } }.
 
-Equations snoc {A: Type} : s A -> A -> s A :=
-snoc (T (Small buf)) x :=
-  T (buffer_snoc buf x);
-snoc (T (G (Green p1 child s1) k)) x :=
-  yellow p1 child (green_suffix_snoc s1 x) k;
-snoc (T (Y (Yellow p1 child s1) k)) x :=
-  let 'Any s1 := yellow_suffix_snoc (Yellowish s1) x in
-  red p1 child s1 k.
+Equations snoc {A: Type} (sq : s A) (x : A) :
+  { sq' : s A | s_seq sq' = s_seq sq ++ [x] }
+:=
+snoc (T (Small buf)) x with buffer_snoc buf x => {
+  | ? buf' => ? T buf' };
+snoc (T (G (Green p1 child s1) k)) x with green_suffix_snoc s1 x => {
+  | ? buf' with yellow p1 child buf' k => {
+    | ? sq' => ? sq' } };
+snoc (T (Y (Yellow p1 child s1) k)) x
+  with yellow_suffix_snoc (Yellowish s1) x => {
+  | ? (Any s1') with red p1 child s1' k => {
+    | ? sq' => ? sq' } }.
 
-Equations uncons {A: Type} (dq: s A) : option (A * s A) :=
-uncons (T (Small buf)) with (buffer_uncons buf) => {
-  uncons _ None := None;
-  uncons _ (Some (x, Any buf')) := Some (x, T (Small buf'))
+Equations uncons {A: Type} (sq : s A) :
+  { o : option (A * s A) |
+    s_seq sq = match o with
+               | None => []
+               | Some (x, sq') => x :: s_seq sq'
+               end } :=
+uncons (T (Small buf)) with buffer_uncons buf => {
+  uncons _ (? None) := ? None;
+  uncons _ (? Some (x, Any buf')) := ? Some (x, T (Small buf'))
 };
-uncons (T (G (Green p1 child s1) k)) :=
-  let '(x, Yellowish p1) := green_uncons p1 in
-  Some (x, yellow p1 child s1 k);
-uncons (T (Y (Yellow p1 child s1) k)) :=
-  let '(x, Any p1) := yellow_uncons (Yellowish p1) in
-  Some (x, red p1 child s1 k).
+uncons (T (G (Green p1 child s1) k)) with green_uncons p1 => {
+  | ? (x, Yellowish p1') with yellow p1' child s1 k => {
+    | ? sq' => ? Some (x, sq') } };
+uncons (T (Y (Yellow p1 child s1) k)) with yellow_uncons (Yellowish p1) => {
+  | ? (x, Any p1') with red p1' child s1 k => {
+    | ? sq' => ? Some (x, sq') } }.
 
-Equations unsnoc {A : Type} (dq: s A) : option (s A * A) :=
-unsnoc (T (Small buf)) with (buffer_unsnoc buf) => {
-  unsnoc _ None := None;
-  unsnoc _ (Some (Any buf', x)) := Some (T (Small buf'), x)
+Equations unsnoc {A : Type} (sq : s A) :
+  { o : option (s A * A) |
+    s_seq sq = match o with
+               | None => []
+               | Some (sq', x) => s_seq sq' ++ [x]
+               end } :=
+unsnoc (T (Small buf)) with buffer_unsnoc buf => {
+  unsnoc _ (? None) := ? None;
+  unsnoc _ (? Some (Any buf', x)) := ? Some (T (Small buf'), x)
 };
-unsnoc (T (G (Green p1 child s1) k)) :=
-  let '(Yellowish s1, x) := green_unsnoc s1 in
-  Some (yellow p1 child s1 k, x);
-unsnoc (T (Y (Yellow p1 child s1) k)) :=
-  let '(Any s1, x) := yellow_unsnoc (Yellowish s1) in
-  Some (red p1 child s1 k, x).
+unsnoc (T (G (Green p1 child s1) k)) with green_unsnoc s1 => {
+  | ? (Yellowish s1', x) with yellow p1 child s1' k => {
+    | ? sq' => ? Some (sq', x) } };
+unsnoc (T (Y (Yellow p1 child s1) k)) with yellow_unsnoc (Yellowish s1) => {
+  | ? (Any s1', x) with red p1 child s1' k => {
+    | ? sq' => ? Some (sq', x) } }.
 
 End S.
 
-Record t (A: Type) := { tlength : Z; tseq : s A }.
+(* Final structure wrapping everything *)
+
+(* There might be a better setup for the definitions; currently the proofs are
+   fairly tedious... *)
+
+Record t (A: Type) : Type := {
+  tlength : Z;
+  tseq : s A;
+  tlength_inv : Z.abs_nat tlength = length (s_seq tseq);
+}.
 Arguments tlength {A}.
 Arguments tseq {A}.
 
-Definition empty {A} : t A :=
-  {| tlength := 0; tseq := T (Small B0) |}.
+Set Equations Transparent.
+Equations t_seq {A} : t A -> list A :=
+t_seq {| tlength := len; tseq := sq |} with Z_lt_le_dec len 0 => {
+  | left _ => rev (s_seq sq)
+  | right _ => s_seq sq
+}.
+Unset Equations Transparent.
 
-Definition is_empty {A} (dq: t A): bool :=
-  tlength dq =? 0.
+Local Ltac case_lt :=
+  match goal with |- context [ Z_lt_le_dec ?x ?y ] =>
+    destruct (Z_lt_le_dec x y); cbn
+  end.
 
-Definition length {A} (dq: t A) : Z :=
-  Z.abs (tlength dq).
+Lemma rev_eq_nil A (l : list A) :
+  rev l = [] -> l = [].
+Proof.
+  intros H%(f_equal (@length _)). cbn in H.
+  rewrite rev_length in H. by apply length_zero_iff_nil.
+Qed.
 
-Definition rev {A} (dq: t A) : t A :=
-  {| tlength := - (tlength dq); tseq := tseq dq |}.
+Local Ltac simplist :=
+  cbn in *;
+  repeat match goal with
+  | H : 0%nat = length ?l |- _ =>
+    symmetry in H; apply length_zero_iff_nil in H; subst
+  | H : rev ?l = [] |- _ =>
+    apply rev_eq_nil in H; subst
+  end.
 
-Definition cons {A} (x: A) (dq: t A) : t A :=
-  let '{| tlength := n; tseq := s |} := dq in
-  if n >=? 0 then
-    {| tlength := n + 1; tseq := S.cons x s |}
-  else
-    {| tlength := n - 1; tseq := S.snoc s x |}.
+Equations empty {A} : { sq : t A | t_seq sq = [] } :=
+empty := ? {| tlength := 0; tseq := T (Small B0) |}.
 
-Definition snoc {A} (dq: t A) (x: A) : t A :=
-  let '{| tlength := n; tseq := s |} := dq in
-  if n >=? 0 then
-    {| tlength := n + 1; tseq := S.snoc s x |}
-  else
-    {| tlength := n - 1; tseq := S.cons x s |}.
+Equations is_empty {A} (sq : t A) :
+  { b : bool | b = true <-> t_seq sq = [] } :=
+is_empty sq := ? (tlength sq =? 0).
+Next Obligation.
+  cbn. intros *.
+  destruct sq as [x s Hlen]. cbn. rewrite Z.eqb_eq. case_lt.
+  all: split; [intros -> | intros HH]; simplist; try hauto.
+  all: rewrite HH /= in Hlen; hauto.
+Qed.
 
-Definition uncons {A} (dq: t A) : option (A * t A) :=
-  let '{| tlength := n; tseq := s |} := dq in
-  if n >=? 0 then
-    match S.uncons s with
-    | None => None
-    | Some (x, s) => Some (x, {| tlength := n-1; tseq := s |})
-    end
-  else
-    match S.unsnoc s with
-    | None => None
-    | Some (s, x) => Some (x, {| tlength := n+1; tseq := s |})
-    end.
+Equations length {A} (sq : t A) :
+  { n : Z | n = Z.of_nat (List.length (t_seq sq)) } :=
+length sq := ? Z.abs (tlength sq).
+Next Obligation.
+  intros. destruct sq as [x s Hlen]. cbn.
+  case_lt; rewrite ?rev_length; lia.
+Qed.
 
-Definition unsnoc {A} (dq: t A) : option (t A * A) :=
-  let '{| tlength := n; tseq := s |} := dq in
-  if n >=? 0 then
-    match S.unsnoc s with
-    | None => None
-    | Some (s, x) => Some ({| tlength := n-1; tseq := s |}, x)
-    end
-  else
-    match S.uncons s with
-    | None => None
-    | Some (x, s) => Some ({| tlength := n+1; tseq := s |}, x)
-    end.
+Equations rev {A} (sq : t A) : { sq' : t A | t_seq sq' = rev (t_seq sq) } :=
+rev {| tlength := n; tseq := s |} :=
+  ? {| tlength := - n; tseq := s |}.
+Next Obligation.
+  cbn. intros ? n s Hlen.
+  case_lt; case_lt; auto; try lia.
+  1: by rewrite rev_involutive //.
+  assert (n = 0) by lia; subst. simplist; hauto.
+Qed.
 
-Definition is_rev {A} (dq: t A) : bool :=
-  tlength dq <? 0.
+Equations cons {A} (x : A) (sq : t A) :
+  { sq' : t A | t_seq sq' = x :: t_seq sq } :=
+cons x {| tlength := n; tseq := s |} with Z_lt_le_dec n 0 => {
+  | right _ with S.cons x s => {
+    | ? s' => ? {| tlength := n + 1; tseq := s' |} };
+  | left _ with S.snoc s x => {
+    | ? s' => ? {| tlength := n - 1; tseq := s' |} }
+}.
+Next Obligation.
+  cbn. intros * ? * -> **. rewrite app_length /=. lia.
+Qed.
+Next Obligation.
+  cbn. intros ? ? ? ? ? ? Hseq Hlen *. case_lt.
+  { rewrite Hseq rev_unit //. }
+  { assert (n = 0) by lia; subst; simplist; hauto. }
+Qed.
+Next Obligation.
+  cbn. intros * ? * Hseq Hlen. rewrite Hseq //=. lia.
+Qed.
+Next Obligation.
+  cbn. intros ? ? ? ? ? ? Hseq Hlen *. case_lt; last hauto.
+  { assert (n = 0) by lia; subst; simplist; hauto. }
+Qed.
+
+Equations snoc {A} (sq : t A) (x : A) :
+  { sq' : t A | t_seq sq' = t_seq sq ++ [x] } :=
+snoc {| tlength := n; tseq := s |} x with Z_lt_le_dec n 0 => {
+  | right _ with S.snoc s x => {
+    | ? s' => ? {| tlength := n + 1; tseq := s' |} };
+  | left _ with S.cons x s => {
+    | ? s' => ? {| tlength := n - 1; tseq := s' |} }
+}.
+Next Obligation. cbn. intros * ? * Hlen * ->. cbn. lia. Qed.
+Next Obligation.
+  cbn. intros ? ? ? ? Hlen ? ? Hseq. case_lt; first hauto.
+  assert (n = 0) by lia; subst; simplist; hauto.
+Qed.
+Next Obligation.
+  cbn. intros * ? * Hlen * ->. rewrite app_length /=. lia.
+Qed.
+Next Obligation.
+  cbn. intros ? ? ? ? Hlen ? ? Hseq. case_lt; last hauto.
+  assert (n = 0) by lia; subst; simplist; hauto.
+Qed.
+
+Equations uncons {A} (sq : t A) :
+  { o : option (A * t A) |
+    t_seq sq = match o with
+               | None => []
+               | Some (x, sq') => x :: t_seq sq'
+               end } :=
+uncons {| tlength := n; tseq := s |} with Z_lt_le_dec n 0 => {
+  | right _ with S.uncons s => {
+    | ? None => ? None;
+    | ? Some (x, s') => ? Some (x, {| tlength := n-1; tseq := s' |})
+  };
+  | left _ with S.unsnoc s => {
+    | ? None => ? None;
+    | ? Some (s', x) => ? Some (x, {| tlength := n+1; tseq := s' |})
+  }
+}.
+Next Obligation.
+  cbn. intros * ? * Hseq%(f_equal (@List.length _)) Hlen.
+  rewrite app_length /= in Hseq. lia.
+Qed.
+Next Obligation.
+  cbn. intros ? ? ? ? ? ? Hseq Hlen. case_lt.
+  { rewrite Hseq rev_unit //. }
+  { assert (n = -1) by lia; subst; simplist.
+    rewrite Hseq rev_unit. rewrite Hseq app_length /= in Hlen.
+    assert (0%nat = List.length (s_seq s')) by lia; simplist. hauto. }
+Qed.
+Next Obligation.
+  cbn. intros * ? * Hseq%(f_equal (@List.length _)) Hlen.
+  cbn in *. lia.
+Qed.
+Next Obligation.
+  cbn. intros ? ? ? ? ? ? Hseq Hlen. case_lt; last hauto.
+  assert (n = 0) by lia; subst; simplist; hauto.
+Qed.
+
+Equations unsnoc {A} (sq : t A) :
+  { o : option (t A * A) |
+    t_seq sq = match o with
+               | None => []
+               | Some (sq', x) => t_seq sq' ++ [x]
+               end } :=
+unsnoc {| tlength := n; tseq := s |} with Z_lt_le_dec n 0 => {
+  | right _ with S.unsnoc s => {
+    | ? None => ? None;
+    | ? Some (s', x) => ? Some ({| tlength := n-1; tseq := s' |}, x)
+  };
+  | left _ with S.uncons s => {
+    | ? None => ? None;
+    | ? Some (x, s') => ? Some ({| tlength := n+1; tseq := s' |}, x)
+  }
+}.
+Next Obligation.
+  cbn. intros * ? * Hseq%(f_equal (@List.length _)) Hlen. hauto.
+Qed.
+Next Obligation.
+  cbn. intros ? ? ? ? ? ? Hseq Hlen. case_lt; first hauto.
+  assert (n = -1) by lia; subst; simplist.
+  rewrite Hseq /=. rewrite Hseq /= in Hlen.
+  assert (0%nat = List.length (s_seq s')) by lia; simplist; hauto.
+Qed.
+Next Obligation.
+  cbn. intros * ? * Hseq%(f_equal (@List.length _)) Hlen.
+  rewrite app_length /= in Hseq. lia.
+Qed.
+Next Obligation.
+  cbn. intros ? ? ? ? ? ? Hseq Hlen. case_lt; last hauto.
+  assert (n = 0) by lia; subst; simplist. rewrite Hlen in Hseq |-*.
+  destruct (s_seq s'); hauto.
+Qed.
+
+Definition is_rev {A} (sq : t A) : bool :=
+  tlength sq <? 0.
